refactored to improve compilation error reporting

I2SFI/Compiler.v
@@ -9,12 +9,18 @@ Require Import Common.Maps.
 Require Import Common.Definitions.
 Require Import Intermediate.Machine.
 Require Import TargetSFI.Machine.
-Require Import TargetSFI.EitherMonad.
-Require Import TargetSFI.StateMonad.
+Require Import CompEitherMonad.
+Require Import CompStateMonad.
 Require Import I2SFI.AbstractMachine.
+
+Require Import TargetSFI.SFIUtil.
+
+Require Import Coq.Strings.String.
 
 Import MonadNotations.
 Open Scope monad_scope.
+
+Definition newline := String "010" ""%string.
 
 (******* Compiler Environment ************)
 
@@ -34,14 +40,13 @@ Record compiler_env : Type :=
     procId2slot : (PMap.t (PMap.t N))
   }.
 
-Notation COMP := (StateMonad.t compiler_env).
-Notation get := (StateMonad.get compiler_env).
-Notation put := (StateMonad.put compiler_env).
-Notation modify := (StateMonad.modify compiler_env).
-Notation "'lift' x" := (StateMonad.lift compiler_env x Coq.Strings.String.EmptyString)
-                         (at level 200).
-Notation fail := (StateMonad.fail compiler_env).
-Notation run := (StateMonad.run compiler_env).
+Notation COMP := (CompStateMonad.t compiler_env).
+Notation get := (CompStateMonad.get compiler_env).
+Notation put := (CompStateMonad.put compiler_env).
+Notation modify := (CompStateMonad.modify compiler_env).
+Notation lift := (CompStateMonad.lift compiler_env).
+Notation fail := (CompStateMonad.fail compiler_env).
+Notation run := (CompStateMonad.run compiler_env).
 
 
 Definition with_current_component (cid : Component.id)
@@ -82,9 +87,11 @@ Definition get_proc_label (cid : Component.id) (pid : Procedure.id)
   do env <- get;
     match (PMap.find cid (exported_procedures_labels env)) with
     | None => fail "Can not find compoent in exported_procedures_labels"
+                  (ExportedProcsLabelsC cid (exported_procedures_labels env))
     | Some cprocs =>
       match (PMap.find pid cprocs) with
       | None => fail "Can not find procedure for component in exported_procedures_labels"
+                    (ExportedProcsLabelsP cid pid (exported_procedures_labels env))
       | Some res => ret res
       end
     end.
@@ -92,15 +99,43 @@ Definition get_proc_label (cid : Component.id) (pid : Procedure.id)
 
 Definition get_sfiId (cid : Component.id) : COMP (SFIComponent.id) :=
   do env <- get;
-    lift (PMap.find cid (cid2SFIid env)).
+    (lift (PMap.find cid (cid2SFIid env))
+          "Missing component id in cid2SFIid"%string
+          (CompEitherMonad.PosArg cid)
+    ).
 
 Definition get_SFI_code_address (cid : Component.id) (pid : Procedure.id)
            (offset : nat) : COMP (RiscMachine.address) :=
   do cenv <- get;
     do sfiId <- get_sfiId cid;      
-    do cmap <- lift (PMap.find cid (procId2slot cenv));
-    do slotid <- lift (PMap.find pid cmap);
+    do cmap <- (lift (PMap.find cid (procId2slot cenv))
+       "Missing component id in procId2slot"%string
+          (CompEitherMonad.PosArg cid));
+    do slotid <- (lift (PMap.find pid cmap)
+       "Missing componentprocedure id in procId2slot"%string
+       (CompEitherMonad.TwoPosArg cid pid));
     ret (SFI.address_of sfiId slotid (N.of_nat offset)). 
+
+Definition get_data_slotid (cid : Component.id) (bid : Block.id)
+  : COMP (N) :=
+  do cenv <- get;
+  do cmap <- lift (PMap.find cid (buffer2slot cenv))
+     "Missing component id in buffer2slot"%string
+     (CompEitherMonad.PosArg cid);
+    lift (PMap.find bid cmap)
+         "Missing block id in buffer2slot"%string
+         (CompEitherMonad.TwoPosArg cid bid).
+      
+
+Definition get_SFI_data_address (cid : Component.id)
+           (bid : Block.id)
+           (offset :  Block.offset)
+  : COMP (RiscMachine.address) :=
+  do cenv <- get;
+    do psfiId <- get_sfiId cid;    
+     do pslotid <- get_data_slotid cid bid;
+    ret (SFI.address_of psfiId pslotid (Z.to_N offset)).
+  
 
 (****************** Initial compiler environment *******************)
 
@@ -162,7 +197,7 @@ Definition init_env (i_cid2SFIid : PMap.t N) (i_procId2slot : PMap.t (PMap.t N))
            (i_next_label : N)
   : compiler_env :=
   {| current_component := 1%positive;
-     next_label := 1%N;
+     next_label := i_next_label;
      buffer2slot := PMap.empty (PMap.t N);
      procId2slot := i_procId2slot;
      exported_procedures_labels := i_exported_procedures_labels;
@@ -206,7 +241,7 @@ Fixpoint allocate_buffers (buffs :  (list (Component.id * (list (Block.id * (nat
                      mem
                      (SFI.address_of sfi_cid (SFI.Allocator.allocator_data_slot) 0%N)
                      (SFI.Allocator.initial_allocator_value (List.length lst)))
-          |_ => fail "allocate_buffers"
+          |_ => fail "allocate_buffers" NoInfo
           end
       end in
   (* components without static buffers *)
@@ -216,8 +251,8 @@ Fixpoint allocate_buffers (buffs :  (list (Component.id * (list (Block.id * (nat
       | cid :: xs =>
         do res_mem <- allocator_init xs mem;
           do cenv <- get;
-          let cid2SFIid := (cid2SFIid cenv) in
-          do sfi_cid <- lift (PMap.find cid cid2SFIid);
+          (* let cid2SFIid := (cid2SFIid cenv) in *)
+          do sfi_cid <-  get_sfiId cid;
            ret (RiscMachine.Memory.set_value
                          res_mem
                          (SFI.address_of sfi_cid (SFI.Allocator.allocator_data_slot) 0%N)
@@ -226,11 +261,10 @@ Fixpoint allocate_buffers (buffs :  (list (Component.id * (list (Block.id * (nat
   do mem1 <- allocate_buffers1 buffs;
     (* need the components without static buffers *)
      do cenv <- get;
-     let cid2SFIid := (cid2SFIid cenv) in
      allocator_init
        (
          List.filter (fun id => (negb (List.existsb (Pos.eqb id) (List.map fst buffs))))
-                     (List.map fst (PMap.elements cid2SFIid))
+                     (List.map fst (PMap.elements (cid2SFIid cenv)))
        ) mem1.
     
 
@@ -255,17 +289,13 @@ Fixpoint init_buffers
           let bid : Block.id := Pointer.block p in
           let offset := Pointer.offset p in    
           if (Z.ltb offset 0%Z)
-          then fail "init_buffers negative offset for pointer"
+          then fail "init_buffers negative offset for pointer" (TwoPosArg cid bid)
           else
             if (Z.leb (Z.of_N SFI.SLOT_SIZE) offset)
             then
-              fail "init_buffers offset too large"
+              fail "init_buffers offset too large" (TwoPosArg cid bid)
             else
-              do cenv <- get;
-              do psfiId <- get_sfiId cid;
-              do cmap <- lift (PMap.find cid (buffer2slot cenv));
-              do pslotid <- lift (PMap.find bid cmap);
-              let address := (SFI.address_of psfiId pslotid (Z.to_N offset)) in
+              do address <- get_SFI_data_address cid bid offset;
               init_buffer 
                 (RiscMachine.Memory.set_value
                    mem
@@ -276,7 +306,8 @@ Fixpoint init_buffers
         end
       end in
                 
-  let fix init_buffers_comp mem cid (lst : (list (Block.id * (nat + list value))))  : COMP (RiscMachine.Memory.t) :=
+  let fix init_buffers_comp mem cid (lst : (list (Block.id * (nat + list value))))
+      : COMP (RiscMachine.Memory.t) :=
       match lst with
       | nil => ret mem
       | (bid,elt)::xs =>
@@ -284,9 +315,8 @@ Fixpoint init_buffers
         | inl _ => ret mem
         | inr vals =>
           do cenv <- get;
-            do sfi_cid <- get_sfiId cid;
-            do cmap <- lift (PMap.find cid (buffer2slot cenv));
-            do slotid <- lift (PMap.find bid cmap);
+            do sfi_cid <- get_sfiId cid;           
+            do slotid <- get_data_slotid cid bid;
             do mem' <- init_buffer mem sfi_cid slotid
                (List.combine (List.seq 0 (List.length vals)) vals);
             init_buffers_comp mem' cid xs
@@ -303,12 +333,15 @@ Fixpoint init_buffers
 
 (******************************** Instruction translation **************************)
 
-Definition sfi_top_address (rd : RiscMachine.Register.t) (cid : SFIComponent.id) : AbstractMachine.code :=
+Definition sfi_top_address (rd : RiscMachine.Register.t)
+           (cid : SFIComponent.id) : AbstractMachine.code :=
   [
-    AbstractMachine.IConst (RiscMachine.to_value (SFI.or_data_mask SFI.MONITOR_COMPONENT_ID))
-                           RiscMachine.Register.R_OR_DATA_MASK
-    ; AbstractMachine.IConst (RiscMachine.to_value (SFI.OFFSET_BITS_NO + SFI.COMP_BITS_NO + 1%N))
-                             rd                           
+    AbstractMachine.IConst
+      (RiscMachine.to_value (SFI.or_data_mask SFI.MONITOR_COMPONENT_ID))
+      RiscMachine.Register.R_OR_DATA_MASK
+    ; AbstractMachine.IConst
+        (RiscMachine.to_value (SFI.OFFSET_BITS_NO + SFI.COMP_BITS_NO + 1%N))
+        rd                           
     ; AbstractMachine.IBinOp (RiscMachine.ISA.ShiftLeft) 
                              RiscMachine.Register.R_SFI_SP
                              rd
@@ -339,8 +372,8 @@ Definition gen_push_sfi (cid : SFIComponent.id) : AbstractMachine.code :=
 Definition gen_pop_sfi (rd : RiscMachine.Register.t) : COMP(AbstractMachine.code) :=
   do cenv <- get;
     do cid <- get_sfiId (current_component cenv);
-    let lbl := ((current_component cenv),(next_label cenv)) in
     do! modify (with_next_label);
+    let lbl := ((current_component cenv),(next_label cenv)) in
       ret
         ( [
             AbstractMachine.ILabel lbl
@@ -380,58 +413,55 @@ Definition compile_IConst
     let cid : Component.id := Pointer.component p in
     let bid : Block.id := Pointer.block p in
     let offset := Pointer.offset p in    
-    if (Z.ltb offset 0%Z) then fail "compile_IConst negative offset for pointer"
+    if (Z.ltb offset 0%Z)
+    then fail "compile_IConst negative offset for pointer " (TwoPosArg cid bid)
     else
       if (Z.leb (Z.of_N SFI.SLOT_SIZE) offset)
-      then fail "compile_IConst offset too large"
+      then fail "compile_IConst offset too large"  (TwoPosArg cid bid)
       else
-        do cenv <- get;
-      do sfiId <- get_sfiId (current_component cenv);
-        match PMap.find cid (buffer2slot cenv) with
-        | None => fail "compile_IConst no cid in buffer2slot"
-        | Some cmap =>
-          match PMap.find bid cmap with
-          | None => fail "compile_IConst no bid in buffer2slot"
-          | Some slotid =>
-            let address := (SFI.address_of sfiId slotid (Z.to_N offset)) in
-            ret [AbstractMachine.IConst (RiscMachine.to_value address) reg']
-          end
-
-      end
+        do address <- get_SFI_data_address cid bid offset;
+        ret [AbstractMachine.IConst (RiscMachine.to_value address) reg']
   end.
 
 Definition compile_IStore (rp : Intermediate.Machine.register)
-           (rs : Intermediate.Machine.register) : COMP (AbstractMachine.code) :=
+           (rs : Intermediate.Machine.register)
+  : COMP (AbstractMachine.code) :=
   ret [
-      AbstractMachine.IBinOp (RiscMachine.ISA.BitwiseAnd)
-                             (map_register rp) (RiscMachine.Register.R_AND_DATA_MASK)
-                             (RiscMachine.Register.R_D)
-      ; AbstractMachine.IBinOp (RiscMachine.ISA.BitwiseOr)
-                             (RiscMachine.Register.R_D) (RiscMachine.Register.R_OR_DATA_MASK)
-                             (RiscMachine.Register.R_D)
-      ; AbstractMachine.IStore (RiscMachine.Register.R_D) (map_register rs)
+      AbstractMachine.IBinOp
+        (RiscMachine.ISA.BitwiseAnd)
+        (map_register rp)
+        (RiscMachine.Register.R_AND_DATA_MASK)
+        (RiscMachine.Register.R_D)
+      ; AbstractMachine.IBinOp
+          (RiscMachine.ISA.BitwiseOr)
+          (RiscMachine.Register.R_D)
+          (RiscMachine.Register.R_OR_DATA_MASK)
+          (RiscMachine.Register.R_D)
+      ; AbstractMachine.IStore
+          (RiscMachine.Register.R_D)
+          (map_register rs)
     ].
-(* Binop r_d <- r_p & r_and_data_mask  *)
-(* Binop r_d <- r_d | r_or_data_mask(cid) *)
-(* Store *r_d <- r_s *)
 
 Definition compile_IJump (rt : Intermediate.Machine.register)
   : COMP (AbstractMachine.code) :=
   ret [
-      AbstractMachine.IBinOp (RiscMachine.ISA.BitwiseAnd)
-                             (map_register rt) (RiscMachine.Register.R_AND_CODE_MASK)
-                             (RiscMachine.Register.R_T)
-      ; AbstractMachine.IBinOp (RiscMachine.ISA.BitwiseOr)
-                             (RiscMachine.Register.R_T) (RiscMachine.Register.R_OR_CODE_MASK)
-                             (RiscMachine.Register.R_T)
-      ; AbstractMachine.IStore (RiscMachine.Register.R_T) (map_register rt)
+      AbstractMachine.IBinOp
+        (RiscMachine.ISA.BitwiseAnd)
+        (map_register rt)
+        (RiscMachine.Register.R_AND_CODE_MASK)
+        (RiscMachine.Register.R_T)
+      ; AbstractMachine.IBinOp
+          (RiscMachine.ISA.BitwiseOr)
+          (RiscMachine.Register.R_T)
+          (RiscMachine.Register.R_OR_CODE_MASK)
+          (RiscMachine.Register.R_T)
+      ; AbstractMachine.IJump (RiscMachine.Register.R_T)
     ].
 
-(* TODO: Either use R_ONE or get rid of it *)
 Definition compile_IAlloc (rp : Intermediate.Machine.register)
            (rs : Intermediate.Machine.register) : COMP (AbstractMachine.code) :=
   do cenv <- get;
-    do cid <- lift (PMap.find (current_component cenv) (cid2SFIid cenv));
+    do cid <- get_sfiId (current_component cenv);
     let rp' := (map_register rp) in
     let rs' := (map_register rs) in
     let (r1,r2) :=
@@ -466,12 +496,6 @@ Definition compile_IAlloc (rp : Intermediate.Machine.register)
       (*   Store *r₂ <- r₁ *)
       ; AbstractMachine.IStore r2  r1
     
-      (* (*   Const r₂ <- 1 *) *)
-      (* ; AbstractMachine.IConst (1%Z) r2 *)
-
-      (* (*   Binop r₁ <- r₁ - r₂ *) *)
-      (* ;  AbstractMachine.IBinOp (RiscMachine.ISA.Subtraction) r1  r2  r1 *)
-                              
       (* # calculate address (s=2*k+1,c,o=0) in r₁ *)      
       (*   Const r₂ <- N+S+1 *)
       ; AbstractMachine.IConst (RiscMachine.to_value (SFI.OFFSET_BITS_NO + SFI.COMP_BITS_NO + 1%N))
@@ -493,25 +517,27 @@ Definition compile_IAlloc (rp : Intermediate.Machine.register)
 
 Definition compile_IReturn : COMP (AbstractMachine.code) :=
   do res <- gen_pop_sfi RiscMachine.Register.R_RA;
-    ret (res ++ [AbstractMachine.IJump RiscMachine.Register.R_RA]).
+    ret (res
+           ++ [
+               AbstractMachine.IJump RiscMachine.Register.R_RA]).
 
-Definition compile_ICall (cid' : Component.id) (pid : Procedure.id)
+Definition compile_ICall (cid1 : Component.id) (pid : Procedure.id)
   : COMP (AbstractMachine.code) :=
   do cenv <- get;
-    do cid <- lift (PMap.find (current_component cenv) (cid2SFIid cenv));
+    do cid <- get_sfiId (current_component cenv);
     let data_mask := RiscMachine.to_value (SFI.or_data_mask cid) in
     let code_mask := RiscMachine.to_value (SFI.or_code_mask cid) in
-    do c'lbl <- get_proc_label cid' pid;
-      let lbl :=  ((current_component cenv),(next_label cenv)) in
+    do clbl <- get_proc_label cid1 pid;
       do! modify (with_next_label);
+      let lbl :=  ((current_component cenv),(next_label cenv)) in
         ret [
-      AbstractMachine.IJal c'lbl
-      ; AbstractMachine.ILabel lbl (* use this to force the next 4 intruction uninterrupted *)
-      ; AbstractMachine.IConst data_mask RiscMachine.Register.R_OR_DATA_MASK
-      ; AbstractMachine.IConst code_mask RiscMachine.Register.R_OR_CODE_MASK
-      ; AbstractMachine.IConst data_mask RiscMachine.Register.R_D
-      ; AbstractMachine.IConst code_mask RiscMachine.Register.R_T
-    ].
+            AbstractMachine.IJal clbl
+            ; AbstractMachine.ILabel lbl (* use this to force the next 4 intruction uninterrupted *)
+            ; AbstractMachine.IConst data_mask RiscMachine.Register.R_OR_DATA_MASK
+            ; AbstractMachine.IConst code_mask RiscMachine.Register.R_OR_CODE_MASK
+            ; AbstractMachine.IConst data_mask RiscMachine.Register.R_D
+            ; AbstractMachine.IConst code_mask RiscMachine.Register.R_T
+          ].
 
 
 Fixpoint compile_instructions (ilist : Intermediate.Machine.code)
@@ -521,7 +547,8 @@ Fixpoint compile_instructions (ilist : Intermediate.Machine.code)
         let cid := (current_component cenv) in
         match i with
         | Intermediate.Machine.INop => ret [AbstractMachine.INop]
-        | Intermediate.Machine.ILabel lbl => ret [AbstractMachine.ILabel (cid,N.pos lbl)]
+        | Intermediate.Machine.ILabel lbl =>
+          ret [AbstractMachine.ILabel (cid, N.of_nat (Pos.to_nat lbl))]
         | Intermediate.Machine.IConst imval reg => (compile_IConst imval reg)
         | Intermediate.Machine.IMov rs rd => ret [AbstractMachine.IMov
                                                    (map_register rs)
@@ -536,9 +563,9 @@ Fixpoint compile_instructions (ilist : Intermediate.Machine.code)
         | Intermediate.Machine.IStore rp rs => (compile_IStore rp rs)
         | Intermediate.Machine.IAlloc rp rs => (compile_IAlloc rp rs)
         | Intermediate.Machine.IBnz r lbl => ret [AbstractMachine.IBnz (map_register r)
-                                                                      (cid,N.pos lbl)]
+                                                                      (cid,N.of_nat (Pos.to_nat lbl))]
         | Intermediate.Machine.IJump rt => (compile_IJump rt)
-        | Intermediate.Machine.IJal lbl => ret [AbstractMachine.IJal (cid,N.pos lbl)]
+        | Intermediate.Machine.IJal lbl => ret [AbstractMachine.IJal (cid,N.of_nat (Pos.to_nat lbl))]
         | Intermediate.Machine.ICall c p => (compile_ICall c p)
         | Intermediate.Machine.IReturn => (compile_IReturn)
         | Intermediate.Machine.IHalt => ret [AbstractMachine.IHalt]
@@ -560,7 +587,8 @@ Definition compile_procedure
   (* if the procedure is exported then must add the sfi stuff*)
   do cenv <- get;
     let cid := (current_component cenv) in
-    do comp_interface <- lift (PMap.find cid interface);
+    do comp_interface <- lift (PMap.find cid interface)
+       "Can't find interface for component " (PosArg cid);
       let exported_procs := Component.export comp_interface in
       let is_exported := List.existsb (Pos.eqb pid) exported_procs in
       do acode <- compile_instructions code; 
@@ -574,6 +602,48 @@ Definition compile_procedure
                   ++ acode )
         else
           ret acode.
+
+Definition check_component_labels (cid : Component.id)
+           (procs : list (Procedure.id * AbstractMachine.code))
+  : COMP(list (Procedure.id * AbstractMachine.code)) :=
+  (* no duplication in labels *)
+  (* exported proc label in offset 1 *)
+  let check_label_duplication (cid:Component.id) procs :=
+      let all_labels :=
+          (List.fold_left
+             (fun acc linstr =>
+                List.fold_left
+                  (fun acc' i =>
+                     match i with
+                     | AbstractMachine.ILabel l => l::acc'
+                     | _ => acc'
+                     end
+                  )
+                  linstr acc                                                                   
+             )
+             procs [] )
+      in
+      if (Nat.eqb (List.length all_labels)
+                  (List.length (List.nodup label_eq_dec all_labels)))
+      then ret procs
+      else fail " check_component_labels::label duplication in component" NoInfo
+  in
+      
+  let check_procedure cid pid acode :=      
+      match acode with
+      | _::(AbstractMachine.ILabel _)::_ => ret procs
+      | _ => fail " check_component_labels::procedure label not found at offset" NoInfo
+      end in
+  
+  let fix check_component cid procs :=
+      match procs with
+      | nil => ret procs
+      | (pid,acode)::xs =>
+        do x <- check_procedure cid pid acode;
+          check_component cid xs
+      end in
+
+  check_component cid procs.
 
 
 Fixpoint compile_components (components : list (Component.id * PMap.t Intermediate.Machine.code))
@@ -593,9 +663,10 @@ Fixpoint compile_components (components : list (Component.id * PMap.t Intermedia
   | [] => ret []
   | (cid,procs)::xs =>
     do! modify (with_current_component cid);
-    do procs <- compile_procedures (PMap.elements procs) interface;
-    do res <- compile_components xs interface;
-    ret ((cid, PMapExtra.of_list procs)::res)
+      do procs <- compile_procedures (PMap.elements procs) interface;
+      do x <- check_component_labels cid procs;
+      do res <- compile_components xs interface;
+      ret ((cid, PMapExtra.of_list procs)::res)
   end.
 
 (*************** Code Alligment and ILabel Removal  *******************)
@@ -607,45 +678,111 @@ use crt to go over list
   if crt address is okay add pair (label,address) to the list
   if not padd with INop until address okay and do the above
 *)
-Definition layout_procedure (cid : Component.id)
-           (pid : Procedure.id) (code : AbstractMachine.code)
-  : COMP ( AbstractMachine.lcode) :=
+Definition layout_procedure
+           (cid : Component.id)
+           (pid : Procedure.id)
+           (plbl : AbstractMachine.label)
+           (code : AbstractMachine.code)
+  : ( AbstractMachine.lcode) :=
+  let padd acc elt :=
+      (* must padd *)
+      (* padd code_lst up to a multiple of SFI.BASIC_BLOCK_SIZE *)
+      let r := N.modulo (N.of_nat (List.length acc))
+                        SFI.BASIC_BLOCK_SIZE in
+      let p := N.modulo (SFI.BASIC_BLOCK_SIZE - r)%N
+                        SFI.BASIC_BLOCK_SIZE in
+      acc
+        ++ (List.repeat
+              (None,AbstractMachine.INop)
+              (N.to_nat p))
+        ++ [elt] in
   
-  do plbl <- (get_proc_label cid pid);
-    ret (snd
-           (List.fold_left
-              (fun (acc:(option (list AbstractMachine.label))*AbstractMachine.lcode)
-                 (i:AbstractMachine.ainstr) =>
-                 
-                 let '(prev_label,code_lst) := acc in
-                 match i with
-                 | AbstractMachine.ILabel lbl =>
-                   if (label_eqb lbl plbl)
-                   then 
-                     (Some [lbl],code_lst)
-                   else                   
-                     match prev_label with
-                     | None =>
-                       (* padd code_lst up to a multiple of SFI.BASIC_BLOCK_SIZE *)
-                       let r := N.modulo (N.of_nat (List.length code_lst))
-                                         SFI.BASIC_BLOCK_SIZE in
-                       let p := N.modulo (SFI.BASIC_BLOCK_SIZE - r)
-                                         SFI.BASIC_BLOCK_SIZE in
-                       let new_code_lst := code_lst
-                                             ++ (List.repeat
-                                                   (None,AbstractMachine.INop)
-                                                   (N.to_nat p)) in
-                       (Some [lbl] ,new_code_lst)
-                     | Some llst => (Some (llst ++ [lbl]),code_lst)
-                     end
-                 | _ => (None,code_lst++[(prev_label,i)])
-                 end
-              ) (code ++ [AbstractMachine.IHalt])
-              (None,
-               @nil ((option (list AbstractMachine.label)) *
-                                AbstractMachine.ainstr))
-           )
-        ).
+  (* accumulate labels *)
+  let lcode1 :=
+      List.map
+        (fun '(ll,i) =>
+           match ll with
+           | nil => (None,i)
+           | _ => (Some ll,i)
+           end
+        )           
+        (snd ( List.fold_left
+            (fun acc elt =>
+               let '(current_labels,lcode) := acc in
+               match elt with
+               | AbstractMachine.ILabel lbl => (current_labels++[lbl],lcode)
+               | _ => (nil,lcode ++ [(current_labels,elt)])
+               end
+            ) code (nil,nil)
+        )) in
+  (* padding *)
+      List.fold_left
+         (fun acc elt =>       
+            match elt with
+            | (None, i) => acc ++ [elt]
+            | (Some ll, i) =>
+              match ll with
+              | nil => acc ++ [elt]
+              | lbl::nil =>
+                if (label_eqb lbl plbl)
+                then
+                  acc ++ [elt]
+                else
+                  padd acc elt
+              | _ =>  padd acc elt
+                
+              end
+            end
+         ) lcode1 nil.
+
+
+Definition check_label_duplication (cid:Component.id)
+           (procs : PMap.t AbstractMachine.lcode) :=
+  let all_labels :=
+      (PMap.fold
+         (fun pid lcode acc =>
+            List.fold_left
+              (fun acc' linstr =>
+                 match linstr with
+                 | (Some ll,_) => acc'++ll
+                 | (None,_) => acc'
+                 end)
+              lcode acc
+         ) procs []) in
+  Nat.eqb (List.length all_labels)
+          (List.length (List.nodup label_eq_dec all_labels)).
+         
+
+Definition check_labeled_code ( labeled_code : (PMap.t (PMap.t AbstractMachine.lcode)))
+  : COMP( (PMap.t (PMap.t AbstractMachine.lcode)) ) :=
+  let check_procedure cid pid lcode :=
+      do l <- get_proc_label cid pid;        
+        match lcode with
+        | _::(Some [lbl],_)::_ => ret  labeled_code
+        | _ => fail " check_labeled_code::procedure label not found at offset "
+                   (DuplicatedLabels labeled_code)
+        end in
+  let fix check_component cid procs :=
+      match procs with
+      | nil => ret  labeled_code
+      | (pid,lcode)::xs =>
+        do x <- check_procedure cid pid lcode;
+          check_component cid xs
+      end in
+  let fix check_progr comps :=
+      match comps with
+      | nil => ret  labeled_code
+      | (cid,comp)::xs =>
+        do x <- check_component cid (PMap.elements comp);
+          if (check_label_duplication cid comp)
+          then
+            check_progr xs
+          else
+            fail " check_labeled_code::label duplication in component "
+                 (DuplicatedLabels labeled_code)
+      end in
+  check_progr (PMap.elements labeled_code).
+
 
 (* acode: cid -> pid -> list of instr (labeled individually) *)
 Definition layout_code (acode : PMap.t (PMap.t AbstractMachine.code))
@@ -659,7 +796,8 @@ Definition layout_code (acode : PMap.t (PMap.t AbstractMachine.code))
         | [] => ret (PMap.empty AbstractMachine.lcode)
         | (pid,code)::xs =>
           do res_map <- layout_procedures cid xs;
-            do acode <- layout_procedure cid pid code;
+              do plbl <- (get_proc_label cid pid);
+            let acode := layout_procedure cid pid plbl code in
             ret (PMap.add pid acode res_map)
         end
   in
@@ -672,7 +810,11 @@ Definition layout_code (acode : PMap.t (PMap.t AbstractMachine.code))
           do proc_res <- layout_procedures cid (PMap.elements procs_map); 
           ret (PMap.add cid proc_res res_map)
       end
-  in  aux (PMap.elements acode).
+  in
+  do lcode <- aux (PMap.elements acode);
+    check_labeled_code lcode.
+
+
 
 
 (********************* Generate code memory and E **********************)
@@ -699,10 +841,10 @@ Definition get_E (lcode : PMap.t (PMap.t AbstractMachine.lcode)) : COMP (Env.E) 
       | [] => ret acc
       | (pid,lbl) :: xs =>        
         match PMap.find cid lcode with
-        | None => fail "get_E did not find component in lcode"
+        | None => fail "get_E did not find component in lcode" (PosArg cid)
         | Some procs_lmap =>
           match PMap.find pid procs_lmap with
-          | None => fail "get_E did not find procedure in lcode"
+          | None => fail "get_E did not find procedure in lcode" (TwoPosArg cid pid)
           | Some listing =>
             let i := index_of lbl listing in
             if (ltb i (List.length listing))
@@ -710,6 +852,7 @@ Definition get_E (lcode : PMap.t (PMap.t AbstractMachine.lcode)) : COMP (Env.E) 
               do address <- get_SFI_code_address cid pid i;
                 (fold_procs cid xs ((address,pid)::acc))
             else fail "get_E the label exported by this procedure is not found in the listing"
+                      (TwoPosArg cid pid)
           end
         end
       end in
@@ -770,47 +913,6 @@ Definition label2address (lc : PMap.t (PMap.t AbstractMachine.lcode))
               (PMap.empty (PMap.t (list (AbstractMachine.label * RiscMachine.address)))).
 
 
-(* Definition label2address (lc : PMap.t (PMap.t AbstractMachine.lcode)) *)
-(*   : COMP (PMap.t (PMap.t (list (AbstractMachine.label * RiscMachine.address)))) := *)
-
-(*   let fix fold_instr cid pid list_instr *)
-(*           (pacc : nat * (list (AbstractMachine.label * RiscMachine.address))) := *)
-(*       let '(i,acc) := pacc in *)
-(*       match list_instr with *)
-(*       | [] => ret (i,acc) *)
-(*       | (olbls,_)::xs => *)
-(*         do address <- get_SFI_code_address cid pid i; *)
-(*         fold_instr cid pid xs *)
-(*                    (match (olbls) with *)
-(*                      | None => ((i+1)%nat,acc) *)
-(*                      | Some ll =>((i+1)%nat, acc++(List.map (fun l => (l,address)) ll)) *)
-(*                     end) *)
-(*       end in *)
-  
-(*   let fix fold_procs cid procs_lst *)
-(*           (acc : (PMap.t (list (AbstractMachine.label * RiscMachine.address)))) := *)
-(*       do cenv <- get; *)
-(*       match procs_lst with *)
-(*       | [] => ret acc *)
-(*       | (pid,proc_lcode) :: xs => *)
-(*         do (_,res) <- fold_instr cid pid proc_lcode (0%nat,[]); *)
-(*           fold_procs cid xs (PMap.add pid res acc) *)
-(*       end in *)
-        
-(*   let fix fold_comp (clist : list (Component.id*(PMap.t AbstractMachine.lcode))) *)
-(*           (acc : (PMap.t (PMap.t (list (AbstractMachine.label * RiscMachine.address))))) :=       *)
-(*       match clist with *)
-(*       | [] => ret acc *)
-(*       | (cid,pmap)::xs => *)
-(*         do res <- fold_procs cid (PMap.elements pmap) *)
-(*            (PMap.empty (list (AbstractMachine.label * RiscMachine.address))); *)
-(*           fold_comp xs (PMap.add cid res acc) *)
-(*       end in *)
-  
-(*   do cenv <- get; *)
-(*     fold_comp (PMap.elements lc) *)
-(*               (PMap.empty (PMap.t (list (AbstractMachine.label * RiscMachine.address)))). *)
-
 (*************************** Monitor component ****************************************)
 
 Definition get_address (cid : Component.id)
@@ -818,10 +920,10 @@ Definition get_address (cid : Component.id)
            (lbl : AbstractMachine.label)
            (l2a :  (PMap.t (PMap.t (list (AbstractMachine.label * RiscMachine.address)))))
   : COMP (RiscMachine.address) :=
-  do pmap <- lift (PMap.find cid l2a);
-    do pl <- lift (PMap.find pid pmap);
+  do pmap <- lift (PMap.find cid l2a) "get_address:No cid" (PosArg cid);
+    do pl <- lift (PMap.find pid pmap) "get_address:No pid" (TwoPosArg cid pid);
     match (List.find (fun '(l,a) => AbstractMachine.label_eqb l lbl) pl) with
-    | None => fail "get_address"
+    | None => fail "get_address:Address not found" NoInfo
     | Some (_,a) => ret a
     end.
 
@@ -834,7 +936,7 @@ Definition  get_address_by_label
               (List.flat_map (fun pmap => List.map snd (PMap.elements pmap))
                           (List.map snd (PMap.elements l2a)) (* list of PMap *))
   in match (List.find (fun '(l,a) => AbstractMachine.label_eqb l lbl) ll) with
-     | None => fail "get_address_by_label"
+     | None => fail "get_address_by_label" NoInfo
      | Some (_,a) => ret a
      end.
 
@@ -925,7 +1027,7 @@ Definition generate_instruction
                                   mem0 address 
                                   RiscMachine.ISA.IHalt)
     
-  | _ => fail "generate_instruction"
+  | _ => fail "generate_instruction"  NoInfo
   end.
 
 Definition generate_procedure_code
@@ -969,13 +1071,10 @@ Definition generate_code_memory
         do res <- generate_component_code cid pmap l2a acc;
           aux xs res
       end in aux (PMap.elements labeled_code) mem0.
-
+      
+      
 Definition compile_program (ip : Intermediate.program) :=
-  (* : Either (sfi_program) :=  *)
-  (* : Either RiscMachine.Memory.t := *)
-    (* cn maps sfi component id to intermediate component id *)
   let cn := gen_cn (Intermediate.prog_interface ip) in
-   (* cid2SFIid maps intermediate component id to sfi id *)
   let cid2SFIid := List.fold_left
                      (fun acc '(cid,i)  =>
                         PMap.add cid (Env.index2SFIid i) acc)
@@ -989,6 +1088,7 @@ Definition compile_program (ip : Intermediate.program) :=
                         (fun m => List.map (fun '(_,(_,l)) => l) (PMap.elements m))
                         (List.map snd (PMap.elements procs_labels)))
                      1%N in
+  
   let procId2slot := allocate_procedure_slots (Intermediate.prog_procedures ip) in
 
   
