I2SFI/CompilerFunctionalTests.v
@@ -7,8 +7,11 @@ Require Import Coq.Lists.List.
 Require Import CompCert.Events.
 
 Require Import I2SFI.Compiler.
+Require Import I2SFI.AbstractMachine.
 Require Import TargetSFI.EitherMonad.
 Require Import TargetSFI.Machine.
+Require Import CompEitherMonad.
+Require Import CompStateMonad.
 Require Import TargetSFI.CS.
 Require Import Intermediate.Machine.
 Require Import Common.Definitions.
@@ -38,8 +41,8 @@ Definition test (instrs : Intermediate.Machine.code)
         Intermediate.prog_main := (COMP1_ID,PROC1_ID)
       |} in
   match compile_program program with
-  | Left msg => Left msg
-  | Right p =>
+  | CompEitherMonad.Left msg err => EitherMonad.Left msg 
+  | CompEitherMonad.Right p =>
     CS.eval_program (100%nat) p RiscMachine.RegisterFile.reset_all
   end.
 
@@ -47,7 +50,7 @@ Example test_INop :
   exists (pc : RiscMachine.address)
     (mem : RiscMachine.Memory.t) 
     (gen_regs : RiscMachine.RegisterFile.t),
-  test [Intermediate.Machine.INop] = Right (E0,(mem,pc,gen_regs)).
+  test [Intermediate.Machine.INop] = EitherMonad.Right (E0,(mem,pc,gen_regs)).
 Proof.  
   compute. eauto. Qed.
 
@@ -56,7 +59,7 @@ Example test_IConst :
     (mem : RiscMachine.Memory.t) 
     (gen_regs : RiscMachine.RegisterFile.t),
     test [Intermediate.Machine.IConst (IInt 5%Z) R_AUX1] =
-    Right (E0,(mem,pc,gen_regs)) /\
+    EitherMonad.Right (E0,(mem,pc,gen_regs)) /\
     (RiscMachine.RegisterFile.get_register RiscMachine.Register.R_AUX1 gen_regs = Some 5%Z)
 .
 Proof.  
@@ -71,8 +74,7 @@ Example test_IMov :
     ->
     test [Intermediate.Machine.IConst (IInt 5%Z) R_AUX1 
           ;Intermediate.Machine.IMov R_AUX1 R_AUX2] =
-    Right (E0,(mem,pc,gen_regs)).
-   
+    EitherMonad.Right (E0,(mem,pc,gen_regs)).   
 Proof.  
   compute. eauto. Qed.
 
@@ -88,7 +90,7 @@ Example test_IStore :
     test  [Intermediate.Machine.IConst (IPtr (1%positive,1%positive,0%Z) ) R_AUX1 
            ; Intermediate.Machine.IConst (IInt 5%Z) R_AUX2 
            ; Intermediate.Machine.IStore R_AUX1 R_AUX2]  =
-    Right (E0,(mem,pc,gen_regs)).   
+    EitherMonad.Right (E0,(mem,pc,gen_regs)).   
 Proof.  
   compute. eauto. Qed.
 
@@ -107,7 +109,7 @@ Example test_ILoad :
                ; Intermediate.Machine.IMov R_AUX1 R_AUX2
                ; Intermediate.Machine.ILoad R_AUX2 R_AUX1
         ]  =
-    Right (E0,(mem,pc,gen_regs)).   
+    EitherMonad.Right (E0,(mem,pc,gen_regs)).   
 Proof.  
   compute. eauto. Qed.
 
@@ -125,7 +127,7 @@ Example test_IBnz :
                ; Intermediate.Machine.ILoad R_AUX2 R_AUX1
                ; Intermediate.Machine.IConst (IInt 0%Z) R_AUX1
                ; Intermediate.Machine.IBnz R_AUX1 7%positive]  =
-    Right (E0,(mem,pc,gen_regs)).   
+    EitherMonad.Right (E0,(mem,pc,gen_regs)).   
 Proof.  
   compute. eauto. Qed.
 
@@ -136,7 +138,7 @@ Example test_IAlloc_Initial_Value :
     test [
         Intermediate.Machine.INop
       ] =
-    Right (E0,(mem,pc,gen_regs)) /\
+    EitherMonad.Right (E0,(mem,pc,gen_regs)) /\
     (*  expect cid=1 slot=1 offset=0 has value 1 *)    
     ((RiscMachine.Memory.get_value mem (SFI.address_of 1%N 1%N 0%N))
      = Some 1).
@@ -151,7 +153,7 @@ Example test_Alloc :
     test [
         Intermediate.Machine.IAlloc R_AUX1 R_AUX2
       ] =
-    Right (E0,(mem,pc,gen_regs))
+    EitherMonad.Right (E0,(mem,pc,gen_regs))
     /\ ((RiscMachine.Memory.get_value mem (SFI.address_of 1%N 1%N 0%N))
      = Some 2) 
 .
@@ -168,8 +170,208 @@ Example test_IAlloc1 :
         ; Intermediate.Machine.IConst (IInt 5%Z) R_AUX2
         ; Intermediate.Machine.IStore R_AUX1 R_AUX2
          ] =
-    Right (E0,(mem,pc,gen_regs)) 
+    EitherMonad.Right (E0,(mem,pc,gen_regs)) 
     /\ ((RiscMachine.Memory.get_value mem (SFI.address_of 1%N 5%N 0%N)) = Some 5%Z)
 .
 Proof.  
   compute. eauto. Qed.
+
+Example test_layout_procedure :
+  layout_procedure 1%positive 1%positive (1%positive,8%N)
+                   [
+                     AbstractMachine.IHalt
+                     ; AbstractMachine.ILabel (1%positive,8%N)
+                     ; AbstractMachine.IJump RiscMachine.Register.R_SP
+                     ; AbstractMachine.IJump RiscMachine.Register.R_SP
+                   ]
+  =
+  [
+    (None, AbstractMachine.IHalt)
+    ; ( Some [(1%positive,8%N)], AbstractMachine.IJump RiscMachine.Register.R_SP)
+    ; ( None, AbstractMachine.IJump RiscMachine.Register.R_SP)
+  ].
+Proof.
+  compute. eauto. Qed.
+
+
+Example test_layout_procedure1 :
+  layout_procedure 1%positive 1%positive (1%positive,8%N)
+                   [
+                     AbstractMachine.IHalt
+                     ; AbstractMachine.ILabel (1%positive,8%N)
+                     ; AbstractMachine.IJump RiscMachine.Register.R_SP
+                     ; AbstractMachine.IJump RiscMachine.Register.R_SP
+                     ; AbstractMachine.ILabel (1%positive,4%N)
+                     ; AbstractMachine.IJump RiscMachine.Register.R_AUX1
+                     ; AbstractMachine.IJump RiscMachine.Register.R_AUX2
+                   ]
+  =
+  [
+    (None, AbstractMachine.IHalt)
+    ; ( Some [(1%positive,8%N)], AbstractMachine.IJump RiscMachine.Register.R_SP)
+    ; ( None, AbstractMachine.IJump RiscMachine.Register.R_SP)
+    ; ( None, AbstractMachine.INop)
+    ; ( None, AbstractMachine.INop)
+    ; ( None, AbstractMachine.INop)
+    ; ( None, AbstractMachine.INop)
+    ; ( None, AbstractMachine.INop)
+    ; ( None, AbstractMachine.INop)
+    ; ( None, AbstractMachine.INop)
+    ; ( None, AbstractMachine.INop)
+    ; ( None, AbstractMachine.INop)
+    ; ( None, AbstractMachine.INop)
+    ; ( None, AbstractMachine.INop)
+    ; ( None, AbstractMachine.INop)
+    ; ( None, AbstractMachine.INop)
+    ; ( Some [(1%positive,4%N)], AbstractMachine.IJump RiscMachine.Register.R_AUX1)
+    ; ( None, AbstractMachine.IJump RiscMachine.Register.R_AUX2)
+  ].
+Proof.
+  compute. eauto. Qed.
+ 
+
+Example test_layout_procedure_no_padding :
+  layout_procedure 1%positive 1%positive (1%positive,8%N)
+                   ( [
+                     AbstractMachine.IHalt
+                     ; AbstractMachine.ILabel (1%positive,8%N)
+                   ]
+                   ++ ( List.repeat (AbstractMachine.IJump RiscMachine.Register.R_SP)
+                                    ((N.to_nat SFI.BASIC_BLOCK_SIZE) - 1) )
+                   ++  [
+                     AbstractMachine.ILabel (1%positive,4%N)
+                     ; AbstractMachine.IJump RiscMachine.Register.R_AUX1
+                     ; AbstractMachine.IJump RiscMachine.Register.R_AUX2
+                   ] )
+  = [
+    (None, AbstractMachine.IHalt)
+    ; ( Some [(1%positive,8%N)], AbstractMachine.IJump RiscMachine.Register.R_SP)
+  ]
+      ++ ( List.repeat
+                 ((None, AbstractMachine.IJump RiscMachine.Register.R_SP))
+                  ((N.to_nat SFI.BASIC_BLOCK_SIZE) - 2) )
+      ++ [ ( Some [(1%positive,4%N)], AbstractMachine.IJump RiscMachine.Register.R_AUX1)
+           ; ( None, AbstractMachine.IJump RiscMachine.Register.R_AUX2)].
+Proof.
+  compute. eauto. Qed.
+
+
+Example exported_procs_labels_test :
+  PMap.equal (PMap.equal label_eqb)
+    ( exported_procs_labels
+        (PMap.add 1%positive
+                  (PMap.add 2%positive
+                            [
+                              Intermediate.Machine.IConst (IInt 1%Z) R_ONE
+                              ; Intermediate.Machine.IJal 1%positive
+                              ; Intermediate.Machine.IHalt
+                            ]
+                  (PMap.add 1%positive
+                            [
+                              Intermediate.Machine.IConst (IInt 1%Z) R_ONE
+                              ; Intermediate.Machine.IJal 1%positive
+                              ; Intermediate.Machine.IReturn
+                              ; Intermediate.Machine.ILabel 1%positive
+                              ; Intermediate.Machine.IMov R_SP R_AUX1
+                              ; Intermediate.Machine.IConst (IInt 20%Z) R_SP
+                              ; Intermediate.Machine.IAlloc R_SP R_SP
+                              ; Intermediate.Machine.IStore R_SP R_AUX1
+                              ; Intermediate.Machine.IBinOp Common.Values.Add R_SP R_ONE R_SP
+                              ; Intermediate.Machine.IConst (IPtr (1%positive,1%positive,0%Z))
+                                                            R_AUX1
+                              ; Intermediate.Machine.ILoad R_AUX1 R_AUX1
+                              ; Intermediate.Machine.IStore R_SP R_AUX1
+                              ; Intermediate.Machine.IBinOp Common.Values.Add R_SP R_ONE R_SP
+                              ; Intermediate.Machine.IConst (IPtr (1%positive,1%positive,0%Z))
+                                                            R_AUX2
+                              ; Intermediate.Machine.IStore R_AUX2 R_COM
+                              ; Intermediate.Machine.IConst (IPtr (1%positive,1%positive,0%Z))
+                                                            R_COM
+                              ; Intermediate.Machine.ILoad R_COM R_COM
+                              ; Intermediate.Machine.IBinOp Common.Values.Minus R_SP R_ONE R_SP
+                              ; Intermediate.Machine.ILoad R_SP R_AUX1
+                              ; Intermediate.Machine.IConst (IPtr (1%positive,1%positive,0%Z))
+                                                            R_AUX2
+                              ; Intermediate.Machine.IStore R_AUX2 R_AUX1
+                              ; Intermediate.Machine.IBinOp Common.Values.Minus R_SP R_ONE R_SP
+                              ; Intermediate.Machine.ILoad R_SP R_SP
+                              ; Intermediate.Machine.IJump R_RA
+                            ]
+                            (PMap.empty Intermediate.Machine.code))
+                  ) (PMap.empty  (PMap.t Intermediate.Machine.code)))
+      (PMap.add 1%positive
+               (Component.mkCompInterface [1%positive;2%positive] [])
+               (PMap.empty Component.interface))
+                  
+    )
+    (
+      (PMap.add 1%positive
+                (PMap.add 2%positive
+                          (1%positive,3%N)
+                 (PMap.add 1%positive
+                           (1%positive,2%N)
+                           (PMap.empty AbstractMachine.label))
+                 ) (PMap.empty  (PMap.t AbstractMachine.label)))
+    ) = true.
+Proof.
+  compute. eauto. Qed.
+
+Example exported_procs_labels_test2 :
+  PMap.equal
+    (PMap.equal label_eqb)
+    ( exported_procs_labels
+        (PMap.add 2%positive                  
+                  (PMap.add 1%positive
+                            [
+                              Intermediate.Machine.IConst (IInt 1%Z) R_ONE
+                              ; Intermediate.Machine.IJal 2%positive
+                              ; Intermediate.Machine.IReturn
+                              ; Intermediate.Machine.ILabel 2%positive
+                              ; Intermediate.Machine.IMov R_SP R_AUX1
+                              ; Intermediate.Machine.IAlloc R_SP R_SP
+                              ; ICall 2%positive 1%positive
+                              ; Intermediate.Machine.IJump R_RA
+                            ]
+                            (PMap.empty Intermediate.Machine.code))
+                  (PMap.add 1%positive
+                            (PMap.add 3%positive
+                                      [
+                                        Intermediate.Machine.IConst (IInt 1%Z) R_ONE
+                                        ; Intermediate.Machine.IJal 1%positive
+                                        ; Intermediate.Machine.IHalt
+                                      ]
+                                      (PMap.add 1%positive
+                                                [
+                                                  Intermediate.Machine.IConst (IInt 1%Z) R_ONE
+                                                  ; Intermediate.Machine.IJal 1%positive
+                                                  ; Intermediate.Machine.IReturn
+                                                  ; Intermediate.Machine.ILabel 1%positive
+                                                  ; Intermediate.Machine.IMov R_SP R_AUX1
+                                                  ; Intermediate.Machine.IAlloc R_SP R_SP
+                                                  ; Intermediate.Machine.IJump R_RA
+                                                ]
+                                                (PMap.empty Intermediate.Machine.code))
+                            ) (PMap.empty  (PMap.t Intermediate.Machine.code))))
+        (PMap.add 2%positive
+                  (Component.mkCompInterface [1%positive] [])
+                  (PMap.add 1%positive
+                            (Component.mkCompInterface [1%positive;3%positive]
+                                                       [(2%positive,1%positive)])
+                            (PMap.empty Component.interface)))                  
+    )
+    (
+      PMap.add 2%positive
+               (PMap.add 1%positive
+                          (2%positive,3%N)
+                          (PMap.empty AbstractMachine.label))
+               (PMap.add 1%positive
+                         (PMap.add 1%positive
+                                   (1%positive,2%N)
+                                   (PMap.add 3%positive
+                                             (1%positive,3%N)
+                                             (PMap.empty AbstractMachine.label)))
+                         (PMap.empty  (PMap.t AbstractMachine.label)))
+    ) = true.
+Proof.
+  compute. eauto. Qed.
+
