I2SFI/CompEitherMonad.v
@@ -1,0 +1,58 @@
+Require Export Lib.Monads.
+Require Import Coq.Strings.String.
+
+Require Import FunctionalExtensionality.
+Require Import AbstractMachine.
+Require Import Common.Maps.
+Require Import Coq.NArith.BinNat.
+
+Set Implicit Arguments.
+
+Inductive CompilerError : Type :=
+| NoInfo : CompilerError
+| DuplicatedLabels :  (PMap.t (PMap.t AbstractMachine.lcode)) -> CompilerError
+| ExportedProcsLabelsC : positive ->  (PMap.t (PMap.t  AbstractMachine.label)) -> CompilerError
+| ExportedProcsLabelsP : positive -> positive ->
+                         (PMap.t (PMap.t  AbstractMachine.label)) -> CompilerError
+| PosArg : positive -> CompilerError
+| TwoPosArg : positive -> positive -> CompilerError
+.
+
+Inductive CompEither {A:Type} : Type :=
+| Right : A -> CompEither
+| Left : string -> CompilerError -> CompEither.
+
+Instance comp_either_monad : Monad (@CompEither)
+  := {
+      
+      ret := fun {A:Type} (x:A) => @Right A x;
+      
+      bind := fun {A B:Type} (x : @CompEither A) (f : A -> @CompEither B) => 
+        match x with
+        | Right y => f y
+        | Left m err => Left m err
+        end
+    }.
+
+Lemma either_monad_left_id:
+  forall A B (a: A) (f: A -> @CompEither B),
+    bind (ret a) f = f a.
+Proof.
+  auto.
+Qed.
+
+Lemma either_monad_right_id:
+  forall A (m: @CompEither A),
+    bind m ret = m.
+Proof.
+  intros.
+  destruct m; auto.
+Qed.
+
+Lemma either_monad_associativity:
+  forall A B C (m: @CompEither A) (f: A -> @CompEither B) (g: B -> @CompEither C),
+    bind (bind m f) g = bind m (fun x => bind (f x) g).
+Proof.
+  intros.
+  destruct m; auto.
+Qed.
