I2SFI/CompStateMonad.v
@@ -1,0 +1,95 @@
+
+Require Export Lib.Monads.
+Require Import Coq.Strings.String.
+
+Require Import FunctionalExtensionality.
+Require Import CompEitherMonad.
+
+Module CompStateMonad.
+  Section Def.
+    Variable st: Type.
+
+    Definition t (res: Type) := st -> (@CompEither res) * st.
+
+    Definition ret (A:Type) (x:A) : (t A)
+      := fun (s:st) => (Right x,s).
+
+    Definition bind A B (s: t A) (f: A -> t B) :=
+      fun x => match s x with
+            | (Right x',s') => (f x') s'
+            | (Left msg err, s') => (Left msg err, s')
+            end.
+
+    Definition get : t st :=
+      fun s => (Right s, s).
+
+    Definition put (s: st) : t unit :=
+      fun _ =>  (Right tt, s).
+
+    Definition modify (f: st -> st) : t unit :=
+      fun s => (Right tt, f s).
+
+    Definition lift {A} (x: option A) (msg : string) (err : CompilerError) : t A :=
+      fun s => match x with
+            | None  => (Left msg NoInfo, s)
+            | Some v => (Right v, s)
+            end.
+    
+    Definition fail {A} (msg : string) (err : CompilerError): t A :=
+      fun s => (Left msg err, s).
+
+    Definition run {A} (s: st) (m: t A) : CompEither :=
+      match m s with
+      | (Left msg err,_) => Left msg err
+      | (Right v,s') => Right v
+      end.
+      
+  End Def.
+End CompStateMonad.
+
+Instance state_monad {st} : Monad (CompStateMonad.t st) := {
+  ret := CompStateMonad.ret st;
+  bind := CompStateMonad.bind st
+}.
+
+Section CompStateMonadLaws.
+  Variable st: Type.
+  
+  Lemma state_monad_left_id:
+    forall res1 res2 (e: res1) (f: res1 -> CompStateMonad.t st res2),
+      bind (ret e) f = f e.
+  Proof.
+    auto.
+  Qed.
+
+  Lemma state_monad_right_id:
+    forall res (m: CompStateMonad.t st res),
+      bind m ret = m.
+  Proof.
+    intros.
+    unfold ret, bind. simpl.
+    unfold CompStateMonad.ret, CompStateMonad.bind.
+    extensionality x.
+    destruct (m x); auto.
+    destruct c. auto. reflexivity. 
+  Qed.
+
+  Lemma state_monad_associativity:
+    forall res1 res2 res3 (m: CompStateMonad.t st res1)
+      (f: res1 -> CompStateMonad.t st res2) (g: res2 -> CompStateMonad.t st res3),
+      bind (bind m f) g = bind m (fun x => bind (f x) g).
+  Proof.
+    intros.
+    unfold ret, bind. simpl.
+    unfold CompStateMonad.ret, CompStateMonad.bind.
+    extensionality x.
+    destruct m; auto.
+    destruct c. destruct (f r s); auto. reflexivity.
+  Qed.
+End CompStateMonadLaws.
+
+Instance state_monad_laws {st} : MonadLaws (CompStateMonad.t st) := {
+  m_left_identity := state_monad_left_id st;
+  m_right_identity := state_monad_right_id st;
+  m_associativity := state_monad_associativity st
+}.
