TargetSFI/SFIUtil.v
@@ -4,6 +4,9 @@
 Require Import List.
 
 Require Import Coq.Structures.Equalities.
+Require Import Coq.Strings.String.
+Require Import Coq.NArith.BinNat.
+Require Import Coq.PArith.BinPos.
 
 Set Implicit Arguments.
 Set Contextual Implicit.
@@ -28,3 +31,46 @@ Module ListUtil.
     end.
    
 End ListUtil.
+
+
+Module Log.
+
+  Open Scope char_scope.
+
+  Definition natToDigit (n : nat) : Ascii.ascii :=
+    match n with
+    | 0 => "0"
+    | 1 => "1"
+    | 2 => "2"
+    | 3 => "3"
+    | 4 => "4"
+    | 5 => "5"
+    | 6 => "6"
+    | 7 => "7"
+    | 8 => "8"
+    | _ => "9"
+  end.
+
+Close Scope char_scope.
+  
+
+  Definition log_nat (n : nat) : string :=
+  let fix log_nat_aux (time n : nat) (acc : string) : string :=
+      let acc' := String (natToDigit (Nat.modulo n 10)) acc in
+      match time with
+      | 0 => acc'
+      | S time' =>
+        match Nat.div n 10 with
+        | 0 => acc'
+        | n' => log_nat_aux time' n' acc'
+        end
+      end in
+  log_nat_aux n n EmptyString.
+
+  Definition log_N (n : N) : string :=
+    log_nat (N.to_nat n).
+
+   Definition log_pos (n : positive) : string :=
+    log_nat (Pos.to_nat n).
+  
+End Log.
